ops done, inj left

proof/rejection_sampling/Ops_LeakageAnalysis.ec
@@ -13,9 +13,10 @@ op sub_step (i : int) : leakages_t =
     LeakAddr [i] ].
 
 
-op sub_g (x : int) : leakages_t.
-axiom sub_g_comp_1 x : x <= 1 => sub_g x = [].
-axiom sub_g_comp_2 x : 1 <  x => sub_g x = sub_step (x-1) ++ sub_g (x - 1).
+op sub_g (x : int) : leakages_t = iteri (x - 1) (fun i r => sub_step (i + 1) ++ r) [].
+lemma sub_g_comp_1 x : x <= 1 => sub_g x = []. by smt(@Int). qed.
+
+lemma sub_g_comp_2 x : 1 <  x => sub_g x = sub_step (x-1) ++ sub_g (x - 1). progress. rewrite /sub_g. smt(@Int). qed.
 
 op sub_f (x : int) : leakages_t = sub_g x ++ sub_prefix.
 
@@ -40,9 +41,13 @@ qed.
 op copy_prefix : leakages_t = LeakFor (0, 32) :: LeakAddr [] ::[].
 op copy_step (i : int) : leakages_t = LeakAddr [i] :: LeakAddr [] :: LeakAddr [i] :: [].
 
-op copy_g (x : int) : leakages_t.
-axiom copy_g_comp_1 x : x <= 0 => copy_g x = [].
-axiom copy_g_comp_2 x : 0 <  x => copy_g x = copy_step (x-1) ++ copy_g (x - 1).
+op copy_g (x : int) : leakages_t = iteri x (fun i r => copy_step i ++ r) [].
+
+lemma copy_g_comp_1 x : x <= 0 => copy_g x = [].
+progress. rewrite /copy_g. smt(@Int). qed.
+
+lemma copy_g_comp_2 x : 0 <  x => copy_g x = copy_step (x-1) ++ copy_g (x - 1).
+progress. rewrite /copy_g. smt(@Int). qed.
 
 op copy_f (x : int) : leakages_t = copy_g x ++ copy_prefix.
 
@@ -65,9 +70,10 @@ qed.
 op dcopy_prefix : leakages_t = LeakFor (0, 64) :: LeakAddr [] ::[].
 op dcopy_step (i : int) : leakages_t = LeakAddr [i] :: LeakAddr [] :: LeakAddr [i] :: [].
 
-op dcopy_g (x : int) : leakages_t.
-axiom dcopy_g_comp_1 x : x <= 0 => dcopy_g x = [].
-axiom dcopy_g_comp_2 x : 0 <  x => dcopy_g x = dcopy_step (x-1) ++ dcopy_g (x - 1).
+
+op dcopy_g (x : int) : leakages_t = iteri x (fun i r => dcopy_step i ++ r) [].
+lemma dcopy_g_comp_1 x : x <= 0 => dcopy_g x = []. by smt(@Int). qed.
+lemma dcopy_g_comp_2 x : 0 <  x => dcopy_g x = dcopy_step (x-1) ++ dcopy_g (x - 1). by smt(@Int). qed.
 
 op dcopy_f (x : int) : leakages_t = dcopy_g x ++ dcopy_prefix.
 
@@ -92,9 +98,9 @@ qed.
 op set0_prefix : leakages_t = LeakFor (0, 32) :: LeakAddr [] :: [].
 op set0_step (i : int) : leakages_t = LeakAddr [i] :: LeakAddr [] :: [].
 
-op set0_g (x : int) : leakages_t.
-axiom set0_g_comp_1 x : x <= 0 => set0_g x = [].
-axiom set0_g_comp_2 x : 0 <  x => set0_g x = set0_step (x-1) ++ set0_g (x - 1).
+op set0_g (x : int) : leakages_t = iteri x (fun i r => set0_step i ++ r) [].
+lemma set0_g_comp_1 x : x <= 0 => set0_g x = []. by smt(@Int). qed.
+lemma set0_g_comp_2 x : 0 <  x => set0_g x = set0_step (x-1) ++ set0_g (x - 1). by smt(@Int). qed.
 
 op set0_f (x : int) : leakages_t = set0_g x ++ set0_prefix.
 
@@ -118,9 +124,9 @@ qed.
 op set1_prefix : leakages_t = LeakFor (1, 32) :: LeakAddr [] :: LeakAddr [0] :: LeakAddr [] :: [].
 op set1_step (i : int) : leakages_t = LeakAddr [i] :: LeakAddr [] :: [].
 
-op set1_g (x : int) : leakages_t.
-axiom set1_g_comp_1 x : x <= 1 => set1_g x = [].
-axiom set1_g_comp_2 x : 1 <  x => set1_g x = set1_step (x-1) ++ set1_g (x - 1).
+op set1_g (x : int) : leakages_t = iteri (x-1) (fun i r => set1_step (i+1) ++ r) [].
+lemma set1_g_comp_1 x : x <= 1 => set1_g x = []. by smt(@Int). qed.
+lemma set1_g_comp_2 x : 1 <  x => set1_g x = set1_step (x-1) ++ set1_g (x - 1). rewrite /set1_g. by smt(@Int). qed.
 
 op set1_f (x : int) : leakages_t = set1_g x ++ set1_prefix.
 
@@ -172,9 +178,9 @@ op swapr_step (x : int) : leakages_t = LeakAddr [x] :: LeakAddr [] :: LeakAddr [
 LeakAddr [x] :: LeakAddr [x] :: LeakAddr [] :: LeakAddr [x] :: 
 LeakAddr [x] :: [].
 
-op swapr_g (x : int) : leakages_t.
-axiom swapr_g_comp_1 x : x = 0 => swapr_g x = [].
-axiom swapr_g_comp_2 x : 0 <  x => swapr_g x = swapr_step (x-1) ++ swapr_g (x - 1).
+op swapr_g (x : int) : leakages_t = iteri x (fun i r => swapr_step i ++ r) [].
+lemma swapr_g_comp_1 x : x = 0 => swapr_g x = []. by smt(@Int). qed.
+lemma swapr_g_comp_2 x : 0 <  x => swapr_g x = swapr_step (x-1) ++ swapr_g (x - 1). by smt(@Int). qed.
 
 op swapr_f (x : int) : leakages_t = swapr_g x ++ swapr_prefix.
 
@@ -206,9 +212,9 @@ LeakAddr [x] :: LeakAddr [] :: [].
 
 op mul1_suffix : leakages_t = LeakAddr [32] :: LeakAddr [] :: LeakAddr [] :: LeakAddr [32] :: [].
 
-op mul1_g (x : int) : leakages_t.
-axiom mul1_g_comp_1 x : x = 1 => mul1_g x = [].
-axiom mul1_g_comp_2 x : 1 <  x => mul1_g x = mul1_step (x-1) ++ mul1_g (x - 1).
+op mul1_g (x : int) : leakages_t  = iteri (x-1) (fun i r => mul1_step (i+1) ++ r) [].
+lemma mul1_g_comp_1 x : x = 1 => mul1_g x = []. by smt(@Int). qed.
+lemma mul1_g_comp_2 x : 1 <  x => mul1_g x = mul1_step (x-1) ++ mul1_g (x - 1). rewrite /mul1_g. smt(@Int). qed.
 
 op mul1_f (x : int) : leakages_t = mul1_suffix ++ mul1_g x ++ mul1_prefix.
 
@@ -227,6 +233,42 @@ rewrite /mul1_f. rewrite (mul1_g_comp_2 (i{hr} +1)).  smt(). simplify. rewrite /
 skip. progress. rewrite /mul1_f.  rewrite mul1_g_comp_1. auto. auto. 
 smt().
 qed.
+
+(* dmul1 LEAKAGES  *)
+op dmul1_prefix : leakages_t = LeakFor (1, 64) :: LeakAddr [] :: LeakAddr [0] :: LeakAddr [] :: LeakAddr [1] :: 
+LeakAddr [] :: LeakAddr [] :: LeakAddr [0] :: LeakAddr [] :: LeakAddr [] :: [].
+op dmul1_step (x : int) : leakages_t = LeakAddr [x] :: LeakAddr [] :: LeakAddr [] :: LeakAddr [] :: LeakAddr
+                                                                   [x] :: 
+LeakAddr [] :: LeakAddr [x + 1] :: LeakAddr [] :: LeakAddr [] :: 
+LeakAddr [x] :: LeakAddr [] :: [].
+
+op dmul1_suffix : leakages_t = LeakAddr [64] :: LeakAddr [] :: LeakAddr [] :: LeakAddr [64] :: [].
+
+op dmul1_g (x : int) : leakages_t = iteri (x-1) (fun i r => dmul1_step (i+1) ++ r) [].
+lemma dmul1_g_comp_1 x : x = 1 => dmul1_g x = []. by smt(@Int). qed.
+lemma dmul1_g_comp_2 x : 1 <  x => dmul1_g x = dmul1_step (x-1) ++ dmul1_g (x - 1). rewrite /dmul1_g. by smt(@Int). qed.
+
+op dmul1_f (x : int) : leakages_t = dmul1_suffix ++ dmul1_g x ++ dmul1_prefix.
+
+lemma dmul1_leakages start_l :
+   hoare [ M(Syscall).dmul1 : M.leakages = start_l 
+     ==> M.leakages = dmul1_f 64 ++ start_l ].
+proof. 
+proc.
+sp.  elim*. progress.
+conseq (_: aux_6 = 64 /\ M.leakages = dmul1_prefix ++ start_l /\ i = 1 ==> _).
+progress. wp.
+while (aux_6 = 64 /\ 1 <= i /\ i <= 64 /\ M.leakages = dmul1_g i ++ dmul1_prefix ++ start_l).
+wp.  skip.  progress. 
+smt(). smt(). 
+rewrite /dmul1_f. rewrite (dmul1_g_comp_2 (i{hr} +1)).  smt(). simplify. rewrite /dmul1_step. simplify. auto.
+skip. progress. rewrite /dmul1_f.  rewrite dmul1_g_comp_1. auto. auto. 
+rewrite /dmul1_f.
+have ->: i0 = 64. smt().
+smt().
+qed.
+
+
 
 
 (* mul1acc LEAKAGES  *)
@@ -252,9 +294,9 @@ LeakAddr [kk + i] :: LeakAddr [] :: LeakAddr [] :: LeakAddr
 LeakAddr [] :: LeakAddr [] :: LeakAddr [] :: LeakAddr [i] :: LeakAddr [] :: [].
 
 
-op mul1acc_g (kk x : int) : leakages_t.
-axiom mul1acc_g_comp_1 kk x : x = 0 => mul1acc_g kk x = [].
-axiom mul1acc_g_comp_2 kk x : 0 < x => mul1acc_g kk x = mul1acc_step kk (x-1) ++ mul1acc_g kk (x - 1).
+op mul1acc_g (kk x : int) : leakages_t =  iteri (x) (fun i r => mul1acc_step kk i ++ r) [].
+lemma mul1acc_g_comp_1 kk x : x = 0 => mul1acc_g kk x = []. smt(@Int). qed.
+lemma mul1acc_g_comp_2 kk x : 0 < x => mul1acc_g kk x = mul1acc_step kk (x-1) ++ mul1acc_g kk (x - 1). smt(@Int). qed.
 
 op mul1acc_f (kk x : int) : leakages_t = mul1acc_suffix kk ++ mul1acc_g kk x ++ mul1acc_prefix.
 
@@ -277,14 +319,67 @@ rewrite /mul1acc_f.
 rewrite /mul1acc_suffix. simplify. auto.
 qed.
 
+
+
+(* dmul1acc LEAKAGES  *)
+op dmul1acc_prefix  : leakages_t = LeakFor (0, 63) :: LeakAddr [] :: LeakAddr [] :: [].
+
+op dmul1acc_suffix (kkk : int) : leakages_t =  LeakAddr [64 +  kkk] :: LeakAddr [] :: LeakAddr [] :: LeakAddr
+                                                               [64 +
+                                                                 kkk] :: 
+LeakAddr [64 +  kkk] :: LeakAddr [] :: LeakAddr [] :: LeakAddr
+                                                               [64 +
+                                                                 kkk] :: 
+LeakAddr [63 +  kkk] :: LeakAddr [] :: LeakAddr [] :: LeakAddr
+                                                               [63 +
+                                                                 kkk] :: 
+LeakAddr [] :: LeakAddr [64 +  kkk] :: LeakAddr [] :: LeakAddr [] :: 
+LeakAddr [63] :: LeakAddr [] :: [].
+
+op dmul1acc_step (kk i : int) : leakages_t = LeakAddr [kk + i + 1] :: LeakAddr [] :: LeakAddr [] :: LeakAddr
+                                                                 [kk +
+                                                                  i + 1] :: 
+LeakAddr [kk + i] :: LeakAddr [] :: LeakAddr [] :: LeakAddr
+                                                             [kk + i] :: 
+LeakAddr [] :: LeakAddr [] :: LeakAddr [] :: LeakAddr [i] :: LeakAddr [] :: [].
+
+
+op dmul1acc_g (kk x : int) : leakages_t =  iteri (x) (fun i r => dmul1acc_step kk i ++ r) [].
+lemma dmul1acc_g_comp_1 kk x : x = 0 => dmul1acc_g kk x = []. smt(@Int). qed.
+lemma dmul1acc_g_comp_2 kk x : 0 < x => dmul1acc_g kk x = dmul1acc_step kk (x-1) ++ dmul1acc_g kk (x - 1). smt(@Int). qed.
+
+op dmul1acc_f (kk x : int) : leakages_t = dmul1acc_suffix kk ++ dmul1acc_g kk x ++ dmul1acc_prefix.
+
+lemma dmul1acc_leakages start_l kkk :
+   hoare [ M(Syscall).dmul1acc : M.leakages = start_l  /\ k = kkk
+     ==> M.leakages = dmul1acc_f (to_uint kkk) 63 ++ start_l ].
+proof. 
+proc.
+sp.  elim*. progress.
+conseq (_: M.leakages = dmul1acc_prefix ++ start_l /\ i = 0 /\ aux = 63 /\ (to_uint kkk) = kk ==> _).
+progress. wp.
+while (aux = 63 /\ 0 <= i /\ i <= 63 /\ M.leakages = dmul1acc_g kk i ++ dmul1acc_prefix ++ start_l /\ kk = (to_uint kkk)).
+wp.  skip.  progress. 
+smt(). smt(). 
+rewrite (dmul1acc_g_comp_2 (to_uint kkk) (i{hr}+1)).  smt(). simplify. rewrite /dmul1acc_step. simplify. auto.
+skip. progress. rewrite dmul1acc_g_comp_1. auto. auto. 
+simplify.
+have -> : i0 = 63. smt().
+rewrite /dmul1acc_f. 
+rewrite /dmul1acc_suffix. simplify. auto.
+qed.
+
+
+
+
 (* bn_muln LEAKAGES  *)
 op bn_muln_prefix : leakages_t = LeakFor (1, 32) :: LeakAddr [] :: (mul1_f 32 ++ [LeakAddr []; LeakAddr [0]]).
 op bn_muln_step (i : int) : leakages_t = mul1acc_f (to_uint ((of_int i))%W64) 31 ++
  [LeakAddr [] ; LeakAddr [] ; LeakAddr [i]] .
 
-op bn_muln_g (x : int) : leakages_t.
-axiom bn_muln_g_comp_1 x : x = 1 => bn_muln_g x = [].
-axiom bn_muln_g_comp_2 x : 1 <  x => bn_muln_g x = bn_muln_step (x-1) ++ bn_muln_g (x - 1).
+op bn_muln_g (x : int) : leakages_t =  iteri (x-1) (fun i r => bn_muln_step  (i+1) ++ r) [].
+lemma bn_muln_g_comp_1 x : x = 1 => bn_muln_g x = []. smt(@Int). qed.
+lemma bn_muln_g_comp_2 x : 1 <  x => bn_muln_g x = bn_muln_step (x-1) ++ bn_muln_g (x - 1). rewrite /bn_muln_g. smt(@Int). qed.
 
 op bn_muln_f (x : int) : leakages_t = bn_muln_g x ++ bn_muln_prefix.
 
@@ -297,11 +392,9 @@ seq 12 : (i = 1 /\ M.leakages = [LeakFor (1, 32) ; LeakAddr [] ] ++ mul1_f 32 ++
 wp. sp. elim*. progress.
 call (mul1_leakages ([LeakAddr [] ; LeakAddr [0] ] ++ start_l)).
 skip. progress. smt(@List).
-
 while (1 <= i /\ i <= 32 /\ M.leakages = bn_muln_g i ++ bn_muln_prefix ++ start_l).
 wp.  
 sp. elim*. progress.
-
 exists* i. elim*. move => i_var.
 call (mul1acc_leakages ([LeakAddr [] ; LeakAddr [] ; LeakAddr [i_var]] ++ leakages) (W64.of_int i_var)).
 skip. progress.
@@ -321,13 +414,55 @@ smt().
 qed.
 
 
+(* dbn_muln LEAKAGES  *)
+op dbn_muln_prefix : leakages_t = LeakFor (1, 64) :: LeakAddr [] :: (dmul1_f 64 ++ [LeakAddr []; LeakAddr [0]]).
+op dbn_muln_step (i : int) : leakages_t = dmul1acc_f (to_uint ((of_int i))%W64) 63 ++
+ [LeakAddr [] ; LeakAddr [] ; LeakAddr [i]] .
+
+op dbn_muln_g (x : int) : leakages_t  =  iteri (x-1) (fun i r => dbn_muln_step  (i+1) ++ r) [].
+lemma dbn_muln_g_comp_1 x : x = 1 => dbn_muln_g x = []. smt(@Int). qed.
+lemma dbn_muln_g_comp_2 x : 1 <  x => dbn_muln_g x = dbn_muln_step (x-1) ++ dbn_muln_g (x - 1). rewrite /dbn_muln_g. smt(@Int). qed.
+
+op dbn_muln_f (x : int) : leakages_t = dbn_muln_g x ++ dbn_muln_prefix.
+
+lemma dbn_muln_leakages start_l :
+   hoare [ M(Syscall).dbn_muln : M.leakages = start_l 
+     ==> M.leakages = dbn_muln_f 64 ++ start_l ].
+proof. 
+proc.
+seq 13 : (aux_3 = 64 /\ i = 1 /\ M.leakages = [LeakFor (1, 64) ; LeakAddr [] ] ++ dmul1_f 64 ++ [LeakAddr []; LeakAddr [0]] ++ start_l).
+wp. sp. elim*. progress.
+call (dmul1_leakages ([LeakAddr [] ; LeakAddr [0] ] ++ start_l)).
+skip. progress. smt(@List).
+while (aux_3 = 64 /\  1 <= i /\ i <= 64 /\ M.leakages = dbn_muln_g i ++ dbn_muln_prefix ++ start_l).
+wp.  
+sp. elim*. progress.
+exists* i. elim*. move => i_var.
+call (dmul1acc_leakages ([LeakAddr [] ; LeakAddr [] ; LeakAddr [i_var]] ++ leakages) (W64.of_int i_var)).
+skip. progress.
+smt().
+smt().
+rewrite (dbn_muln_g_comp_2 (i{hr}+1)). smt(). simplify. rewrite /dbn_muln_step.
+pose xxx := dmul1acc_f (to_uint ((of_int i{hr}))%W64) 63.
+do ? rewrite - catA.
+congr.
+congr. congr. 
+smt(@List).
+skip.
+progress.
+rewrite dbn_muln_g_comp_1. auto. simplify.
+rewrite /dbn_muln_prefix. auto.
+smt().
+qed.
+
+
 (* div2 LEAKAGES  *)
 op div2_prefix (k : int) : leakages_t = LeakFor (0, k) :: LeakAddr [] :: [].
 op div2_step (i : int) : leakages_t = LeakAddr [i] :: LeakAddr [64 + i] :: [].
 
-op div2_g (x : int) : leakages_t.
-axiom div2_g_comp_1 x : x = 0 => div2_g x = [].
-axiom div2_g_comp_2 x : 0 <  x => div2_g x = div2_step (x-1) ++ div2_g (x - 1).
+op div2_g (x : int) : leakages_t   =  iteri x (fun i r => div2_step  i ++ r) [].
+lemma div2_g_comp_1 x : x = 0 => div2_g x = []. smt(@Int). qed.
+lemma div2_g_comp_2 x : 0 <  x => div2_g x = div2_step (x-1) ++ div2_g (x - 1). smt(@Int). qed.
 
 op div2_f (x k : int) : leakages_t = div2_g x ++ div2_prefix k.
 
@@ -353,9 +488,9 @@ qed.
 op bn_shrink_prefix : leakages_t = LeakFor (0, 32) :: LeakAddr [] :: [].
 op bn_shrink_step (i : int) : leakages_t = LeakAddr [i] :: LeakAddr [i] :: [].
 
-op bn_shrink_g (x : int) : leakages_t.
-axiom bn_shrink_g_comp_1 x : x = 0 => bn_shrink_g x = [].
-axiom bn_shrink_g_comp_2 x : 0 <  x => bn_shrink_g x = bn_shrink_step (x-1) ++ bn_shrink_g (x - 1).
+op bn_shrink_g (x : int) : leakages_t =  iteri x (fun i r => bn_shrink_step i ++ r) [].
+lemma bn_shrink_g_comp_1 x : x = 0 => bn_shrink_g x = []. smt(@Int). qed.
+lemma bn_shrink_g_comp_2 x : 0 <  x => bn_shrink_g x = bn_shrink_step (x-1) ++ bn_shrink_g (x - 1). smt(@Int). qed.
 
 op bn_shrink_f (x : int) : leakages_t = bn_shrink_g x ++ bn_shrink_prefix.
 
@@ -387,9 +522,9 @@ op dsub_step (i : int) : leakages_t =
     LeakAddr [i] ].
 
 
-op dsub_g (x : int) : leakages_t.
-axiom dsub_g_comp_1 x : x <= 1 => dsub_g x = [].
-axiom dsub_g_comp_2 x : 1 <  x => dsub_g x = dsub_step (x-1) ++ dsub_g (x - 1).
+op dsub_g (x : int) : leakages_t =  iteri (x-1) (fun i r => dsub_step  (i+1) ++ r) [].
+lemma dsub_g_comp_1 x : x <= 1 => dsub_g x = []. smt(@Int). qed.
+lemma dsub_g_comp_2 x : 1 <  x => dsub_g x = dsub_step (x-1) ++ dsub_g (x - 1). rewrite /dsub_g. smt(@Int). qed.
 
 op dsub_f (x : int) : leakages_t = dsub_g x ++ dsub_prefix.
 
@@ -416,13 +551,13 @@ op bn_expand_prefix : leakages_t = LeakFor (0, 32) :: LeakAddr [] :: [].
 op bn_expand_step (i : int) : leakages_t = LeakAddr [i] :: LeakAddr [i] :: [].
 op bn_expand_step2 (i : int) : leakages_t = LeakAddr [i] :: LeakAddr [] :: [].
 
-op bn_expand_g (x : int) : leakages_t.
-axiom bn_expand_g_comp_1 x : x = 0 => bn_expand_g x = [].
-axiom bn_expand_g_comp_2 x : 0 <  x => bn_expand_g x = bn_expand_step (x-1) ++ bn_expand_g (x - 1).
+op bn_expand_g (x : int) : leakages_t = iteri x (fun i r => bn_expand_step  i ++ r) [].
+lemma bn_expand_g_comp_1 x : x = 0 => bn_expand_g x = []. smt(@Int). qed.
+lemma bn_expand_g_comp_2 x : 0 <  x => bn_expand_g x = bn_expand_step (x-1) ++ bn_expand_g (x - 1). smt(@Int). qed.
 
-op bn_expand_h (x : int) : leakages_t.
-axiom bn_expand_h_comp_1 x : x = 32 => bn_expand_h x = [].
-axiom bn_expand_h_comp_2 x : 32 < x => bn_expand_h x = bn_expand_step2 (x-1) ++ bn_expand_h (x - 1).
+op bn_expand_h (x : int) : leakages_t = iteri (x-32) (fun i r => bn_expand_step2 (i + 32) ++ r) [].
+lemma bn_expand_h_comp_1 x : x = 32 => bn_expand_h x = []. smt(@Int). qed.
+lemma bn_expand_h_comp_2 x : 32 < x => bn_expand_h x = bn_expand_step2 (x-1) ++ bn_expand_h (x - 1). rewrite /bn_expand_h. smt(@Int). qed.
 
 
 op bn_expand_f (x : int) : leakages_t = bn_expand_h (2 * x) ++ [LeakFor (32, 64) ; LeakAddr [] ] ++ bn_expand_g x ++ bn_expand_prefix.
@@ -464,9 +599,9 @@ op dbn_cmov_prefix : leakages_t = LeakFor (0, 64) :: LeakAddr [] :: [].
 op dbn_cmov_step (i : int) : leakages_t = LeakAddr [i] :: LeakAddr [] :: LeakAddr [] :: LeakAddr [i] :: 
 LeakAddr [i] :: [].
 
-op dbn_cmov_g (x : int) : leakages_t.
-axiom dbn_cmov_g_comp_1 x : x = 0 => dbn_cmov_g x = [].
-axiom dbn_cmov_g_comp_2 x : 0 <  x => dbn_cmov_g x = dbn_cmov_step (x-1) ++ dbn_cmov_g (x - 1).
+op dbn_cmov_g (x : int) : leakages_t = iteri (x) (fun i r => dbn_cmov_step (i) ++ r) [].
+lemma dbn_cmov_g_comp_1 x : x = 0 => dbn_cmov_g x = []. smt(@Int). qed.
+lemma dbn_cmov_g_comp_2 x : 0 <  x => dbn_cmov_g x = dbn_cmov_step (x-1) ++ dbn_cmov_g (x - 1). smt(@Int). qed.
 
 op dbn_cmov_f (x : int) : leakages_t = dbn_cmov_g x ++ dbn_cmov_prefix.
 
@@ -514,19 +649,75 @@ auto.
 qed.
 
 (* bn_breduce LEAKAGES  *)
-op bn_breduce_f (x : int) : leakages_t.
+op bn_breduce_f : leakages_t = bn_shrink_f 32 ++ [LeakAddr []] ++ dbn_cmov_g 64 ++ dbn_cmov_prefix ++
+[LeakAddr []] ++ dsub_g 64 ++ dsub_prefix ++ [LeakAddr []] ++ dcopy_g 64 ++
+dcopy_prefix ++ [LeakAddr []] ++ [LeakAddr []] ++ bn_expand_h (2 * 32) ++
+[LeakFor (32, 64); LeakAddr []] ++ bn_expand_g 32 ++ bn_expand_prefix ++
+[LeakAddr []] ++ dsub_g 64 ++ dsub_prefix ++ [LeakAddr []] ++ bn_muln_g 32 ++
+bn_muln_prefix ++ [LeakAddr []] ++ bn_shrink_g 32 ++ bn_shrink_prefix ++
+[LeakAddr []] ++ div2_g 64 ++ div2_prefix 64 ++ [LeakAddr []] ++
+dbn_muln_g 64 ++ dbn_muln_prefix ++ [LeakAddr []].
 
 lemma bn_breduce_leakages start_l :
    hoare [ M(Syscall).bn_breduce : M.leakages = start_l 
-     ==> M.leakages = bn_breduce_f 32 ++ start_l ].
+     ==> M.leakages = bn_breduce_f ++ start_l ].
 proof. 
 proc. 
-admitted.
+pose suf1 :=  [LeakAddr []] ++ start_l.
+seq 13 : (M.leakages = dbn_muln_f 64 ++ suf1 ).
+wp.  call (dbn_muln_leakages suf1). simplify. wp. skip. progress. 
+
+pose suf2 :=  [LeakAddr []] ++ dbn_muln_f 64 ++ suf1.
+seq 3 : (M.leakages = div2_f 64 64 ++ suf2).
+wp.  call (div2_leakages suf2 64). simplify. wp. skip. progress. 
+
+pose suf3 :=  [LeakAddr []] ++ div2_f 64 64 ++ suf2.
+seq 3 : (M.leakages = bn_shrink_f 32 ++ suf3).
+wp.  call (bn_shrink_leakages suf3). simplify. wp. skip. progress. 
+
+pose suf4 :=  [LeakAddr []] ++ bn_shrink_f 32 ++ suf3.
+seq 3 : (M.leakages = bn_muln_f 32 ++ suf4).
+wp.  call (bn_muln_leakages suf4). simplify. wp. skip. progress. 
+
+pose suf5 :=  [LeakAddr []] ++ bn_muln_f 32 ++ suf4.
+seq 7 : (M.leakages = dsub_f 64  ++ suf5).
+wp.  call (dbn_subc_leakages suf5). simplify. wp. skip. progress. 
+
+pose suf6 :=  [LeakAddr []] ++ dsub_f 64 ++ suf5.
+seq 3 : (M.leakages = bn_expand_f 32  ++ suf6).
+wp. call (bn_expand_leakages suf6). simplify. wp. skip. progress. 
+
+pose suf7 :=  [LeakAddr []] ++ bn_expand_f 32 ++ suf6.
+seq 3 : (M.leakages = dcminusP_f   ++ suf7).
+wp. call (dcminusP_leakages suf7). simplify. wp. skip. progress. 
+
+pose suf8 :=  [LeakAddr []] ++ dcminusP_f ++ suf7.
+seq 3 : (M.leakages = bn_shrink_f 32   ++ suf8).
+wp. call (bn_shrink_leakages suf8). wp. skip.
+progress.
+skip. progress.
+rewrite /suf8 /suf7 /suf6 /suf5 /suf4 /suf3 /suf2 /suf1.
+do? rewrite catA.
+auto.
+qed.
 
 (* mulm LEAKAGES  *)
-op mulm_t : leakages_t.
+op mulm_t : leakages_t = bn_breduce_f ++ [LeakAddr []] ++ bn_muln_g 32 ++ bn_muln_prefix ++
+[LeakAddr []] .
 lemma mulm_leakages start_l : 
    hoare [ M(Syscall).mulm : M.leakages = start_l 
                 ==> M.leakages = mulm_t ++ start_l ].
-proof. 
-admitted.
+proof. proc.
+pose suf1 :=  [LeakAddr []] ++ start_l.
+seq 7 : (M.leakages = bn_muln_f 32 ++ suf1 ).
+wp. call (bn_muln_leakages suf1). simplify. wp. skip. progress. 
+
+pose suf2 :=  [LeakAddr []] ++ bn_muln_f 32 ++ suf1.
+seq 3 : (M.leakages = bn_breduce_f ++ suf2).
+wp. call (bn_breduce_leakages suf2). simplify. wp. skip. progress. 
+skip. auto.
+progress.
+rewrite /suf2 /suf1.
+do? rewrite catA.
+auto.
+qed.
